src/program_proof/single/single_proof.v
@@ -1,0 +1,101 @@
+From iris.algebra Require Import gmap lib.mono_nat.
+From iris.proofmode Require Import base tactics classes.
+From iris.bi.lib Require Import fractional.
+From Perennial.program_proof Require Import proof_prelude.
+From Perennial.program_proof.single Require Import replica_proof.
+From Goose.github_com.mit_pdos.gokv.paxi Require Import single.
+
+Section single_proof.
+
+Context `{!heapG Σ}.
+
+Record PrepareReplyC := mkPrepareReplyC
+{
+    Prep_Pn : u64;
+    Prep_Val : u64;
+    Prep_Success : bool;
+}
+.
+Definition own_PrepareReply (reply_ptr:loc) (reply:PrepareReplyC) : iProp Σ :=
+  "HPn" ∷ reply_ptr ↦[PrepareReply :: "Pn"] #reply.(Prep_Pn) ∗
+  "HVal" ∷ reply_ptr ↦[PrepareReply :: "Val"] #reply.(Prep_Val) ∗
+  "HSuccess" ∷ reply_ptr ↦[PrepareReply :: "Success"] #reply.(Prep_Success)
+.
+
+(* TODO: do majority election ghost proof, to give winner of a proposal number
+   ownership of the pn_undec *)
+
+Context `{paxosG Σ u64}.
+Context `{f:nat}.
+
+Definition own_Replica (r:loc) (pid:nat) γ : iProp Σ :=
+  ∃ (promisePN valPN:u64) (v:u64),
+  "HpromisedPN" ∷ r ↦[Replica :: "promisedPN"] #promisePN ∗
+  "HvalPN" ∷ r ↦[Replica :: "valPN"] #valPN ∗
+  "HacceptedVal" ∷ r ↦[Replica :: "acceptedVal"] #v ∗
+  "HcommittedVal" ∷ r ↦[Replica :: "committedVal"] #v ∗
+  "#Hacc_prop" ∷ pn_ptsto f γ (int.nat valPN) v ∗
+  "#Hrej" ∷ (∀ pn', ⌜(int.nat valPN) < pn'⌝ → ⌜pn' ≤ int.nat promisePN⌝ → rejected γ pid pn') ∗
+  "Hundec" ∷ ([∗ set] pn' ∈ (fin_to_set (C:=gset u64) u64), ⌜int.nat pn' ≤ int.nat promisePN⌝ ∨ undecided γ pid (int.nat pn')) ∗
+  "Hvotes" ∷ True
+  (* "Hpeers" ∷ *)
+.
+
+Lemma wp_PrepareRPC (r:loc) γ pid (reply_ptr:loc) (pn:u64) dummy_rep :
+  {{{
+       own_Replica r pid γ ∗
+       own_PrepareReply reply_ptr dummy_rep
+  }}}
+    Replica__PrepareRPC #r #pn #reply_ptr
+  {{{
+       reply, RET #(); own_Replica r pid γ ∗
+            own_PrepareReply reply_ptr reply ∗
+            (⌜reply.(Prep_Success) = false⌝ ∨
+             pn_ptsto f γ (int.nat reply.(Prep_Pn)) (reply.(Prep_Val)) ∗
+             (∀ pn', ⌜pn' < int.nat pn⌝ → ⌜int.nat reply.(Prep_Pn) < pn'⌝ → rejected γ pid pn')
+             )
+  }}}
+.
+Proof.
+  iIntros (Φ) "Hpre HΦ".
+  wp_lam.
+  wp_pures.
+  iDestruct "Hpre" as "[Hown Hrep]".
+  iNamed "Hown".
+
+  wp_loadField.
+  wp_if_destruct.
+  { (* able to make a promise for that key *)
+    wp_storeField.
+    wp_loadField.
+    iNamed "Hrep".
+    wp_storeField.
+    wp_loadField.
+    wp_storeField.
+    wp_storeField.
+    iApply "HΦ".
+    (* XXX: will be annoying to do a ghost update to a range of pns in "Hundec" *)
+    admit.
+  }
+  { (* can't vote for caller *)
+    iNamed "Hrep".
+    wp_storeField.
+    wp_loadField.
+    wp_storeField.
+    iApply "HΦ".
+    iSplitR "HPn HVal HSuccess".
+    {
+      iExists _, _, _.
+      iFrame "∗#".
+    }
+    iSplitR "".
+    {
+      instantiate (1:=(mkPrepareReplyC _ _ _)).
+      iFrame.
+    }
+    simpl.
+    by iLeft.
+  }
+Admitted.
+
+End single_proof.
